theories/Notations.v
@@ -83,9 +83,17 @@ Reserved Notation "P -∗ Q"
   (at level 99, Q at level 200, right associativity,
    format "'[' P  '/' -∗  Q ']'").
 
+Reserved Notation "x != y" (at level 70, no associativity).
+
 Reserved Notation "x +ᵇ y" (at level 50, left associativity).
 Reserved Notation "x -ᵇ y" (at level 50, left associativity).
 Reserved Notation "x *ᵇ y" (at level 40, left associativity).
+
+(* Signed bitvector operations *)
+Reserved Notation "x >=ˢ y" (at level 70, no associativity).
+Reserved Notation "x >ˢ y" (at level 70, no associativity).
+Reserved Notation "x <=ˢ y" (at level 70, no associativity).
+Reserved Notation "x <ˢ y" (at level 70, no associativity).
 
 (* Unsigned bitvector operations *)
 Reserved Notation "x >=ᵘ y" (at level 70, no associativity).
